---
title: "Formulas"
author: "Shinichi Nakagawa"
date: '2022-06-29'
output:
  word_document: default
  html_document: default
---

$$
\ln{\text{RR}} = \ln \left( \frac{m_{T}} {m_{C}}\right) + 
\frac{1}{2} \left(\frac{\text{CV}_T^2} {n_{T}} - \frac{\text{CV}_C^2} {n_{C}}\right), 
$$


$$
v(\ln{\text{RR}}) = \frac{\text{CV}_T^2} {n_{T}} + \frac{\text{CV}_C^2} {n_{C}} +
\frac{\text{CV}_T^4} {2n_{T}^2} + \frac{\text{CV}_C^4} {2n_{C}^2},
$$

$n_{T} = n_{C} = n$

$\text{CV}_C = sd_T/m_T$ and $\text{CV}_C = sd_C/m_C$


$$
\ln{\text{RR}} = \ln \left( \frac{m_{T}} {m_{C}}\right) + 
\frac{1}{2} \left(\frac{\sum_{i=1}^{k}{\text{CV}_{Ti}^2}/k} {n_{T}} - \frac{\sum_{i=1}^{k}{\text{CV}_{Ci}^2}/k} {n_{C}}\right), 
$$

$$
v(\ln{\text{RR}})= \frac{\sum_{i=1}^{k}{\text{CV}_{Ti}^2}/k} {n_{T
}} + \frac{\sum_{i=1}^{k}{\text{CV}_{Ci}^2}/k} {n_{C}} +
\frac{(\sum_{i=1}^{k}{\text{CV}_{Ti}^2}/k)^2} {2n_{T}^2} + 
\frac{(\sum_{i=1}^{k}{\text{CV}_{Ci}^2}/k)^2} {2n_{C}^2} 
$$


$$
f(M) = \arcsin(\sqrt{M})
$$

$$
\text{var}(f(M)) = \frac{1}{8}
$$


$$
\ln{\text{RR}}_{folded} = \sqrt{v(\ln{\text{RR}})\frac{2}{\pi}} \exp\left(-{\frac{\ln{\text{RR}}^2}{2v(\ln{\text{RR}})}}\right)+\ln{\text{RR}}\left[1-2\Phi\left(-\frac{\ln{\text{RR}}}{\sqrt{v(\ln{\text{RR}})}}\right) \right],
$$

$$
v(\ln{\text{RR}})_{folded} = \ln{\text{RR}}^2 + v(\ln{\text{RR}}) - \ln{\text{RR}}_{folded}^2
$$